Update the definition of stateful_key to take a size_t for the length and a meta bool no_key

code/streaming/Hacl.Streaming.Blake2.fst
@@ -144,63 +144,81 @@ inline_for_extraction noextract
 let key_size_ty (a : alg) = key_size:nat{0 <= key_size /\ key_size <= Spec.max_key a}
 
 inline_for_extraction noextract
-let key_size_t (a : alg) = key_size:U32.t{0 <= U32.v key_size /\ U32.v key_size <= Spec.max_key a}
+let key_size_t (a : alg) (is_zero: bool) =
+  key_size:U32.t{
+    0 <= U32.v key_size /\ U32.v key_size <= Spec.max_key a /\
+    (is_zero ==> U32.v key_size = 0)}
 
 /// Defining stateful keys
 inline_for_extraction noextract
-let stateful_key_t (a : alg) (key_size : key_size_ty a) : Type =
-  if key_size = 0 then unit else b:B.buffer uint8 { B.length b == key_size }
+let stateful_key_t (a : alg) (no_key : bool)
+                   (key_size : key_size_t a no_key) : Type =
+  if no_key then unit else b:B.buffer uint8 { B.length b == U32.v key_size}
 
 inline_for_extraction noextract
-let buffer_to_stateful_key_t (a : alg) (key_size : key_size_ty a{key_size > 0})
-                             (k : B.buffer uint8 { B.length k == key_size }) :
-  Tot (stateful_key_t a key_size) =
+let buffer_to_stateful_key_t (a : alg) (key_size : key_size_t a false)
+                             (k : B.buffer uint8 { B.length k == U32.v key_size }) :
+  Tot (stateful_key_t a false key_size) =
   k
 
 inline_for_extraction noextract
 let unit_to_stateful_key_t (a : alg) :
-  Tot (stateful_key_t a 0) =
+  Tot (stateful_key_t a true 0ul) =
   ()
 
-/// Pay attention to the fact that the ``key_size`` parameter is not Low* and
-/// appears in extracted code: it must be a constant.
+/// The ``has_key`` parameter is meta
 /// TODO: this definition could be moved to Hacl.Streaming.Interface, it could
 /// be pretty useful in other situations as it generalizes ``stateful_buffer`` in
 /// the case the length is zero. Note that rather than being unit, the type could
 /// be buffer too (and we would use null whenever needed).
 inline_for_extraction noextract
-let stateful_key (a : alg) (key_size : key_size_ty a) : I.stateful unit =
+let stateful_key (a : alg) (no_key : bool) (key_size : key_size_t a no_key) :
+  I.stateful unit =
   I.Stateful
-    (fun _ -> stateful_key_t a key_size)
-    (fun #_ h s -> if key_size = 0 then B.loc_none else B.loc_addr_of_buffer (s <: B.buffer uint8))
-    (fun #_ h s -> if key_size = 0 then True else B.freeable (s <: B.buffer uint8))
-    (fun #_ h s -> if key_size = 0 then True else B.live h (s <: B.buffer uint8))
-    (fun _ -> s:S.seq uint8 { S.length s == key_size })
-    (fun _ h s -> if key_size = 0 then Seq.empty else B.as_seq h (s <: B.buffer uint8))
-    (fun #_ h s -> ())
-    (fun #_ l s h0 h1 -> ())
-    (fun #_ l s h0 h1 -> ())
+    (fun _ -> stateful_key_t a no_key key_size)
+    (* footprint *)
+    (fun #_ h s -> if U32.v key_size = 0 then B.loc_none else B.loc_addr_of_buffer (s <: B.buffer uint8))
+    (* freeable *)
+    (fun #_ h s -> if U32.v key_size = 0 then True else B.freeable (s <: B.buffer uint8))
+    (* invariant *)
+    (fun #_ h s ->
+      if no_key then True else if U32.v key_size = 0 then (s <: B.buffer uint8) == B.null
+      else B.live h (s <: B.buffer uint8))
+    (fun _ -> s:S.seq uint8 { S.length s == U32.v key_size })
+    (fun _ h s -> if U32.v key_size = 0 then Seq.empty else B.as_seq h (s <: B.buffer uint8))
+    (fun #_ h s -> ()) (* invariant_loc_in_footprint *)
+    (fun #_ l s h0 h1 -> ()) (* frame_invariant *)
+    (fun #_ l s h0 h1 -> ()) (* frame_freeable *)
+
+    (* alloca *)
     (fun () ->
-       if key_size = 0 then unit_to_stateful_key_t a
-       else
-         buffer_to_stateful_key_t a key_size (B.alloca (Lib.IntTypes.u8 0)
-                                                       (U32.uint_to_t key_size)))
-    (fun () r -> 
-      if key_size = 0 then unit_to_stateful_key_t a
-      else
-        buffer_to_stateful_key_t a key_size (B.malloc r (Lib.IntTypes.u8 0)
-                                                        (U32.uint_to_t key_size)))
-    (fun _ s -> if key_size = 0 then () else  B.free (s <: B.buffer uint8))
+       if no_key then unit_to_stateful_key_t a
+       else if U32.(key_size >^ 0ul) then
+         buffer_to_stateful_key_t a key_size (B.alloca (Lib.IntTypes.u8 0) key_size)
+       else buffer_to_stateful_key_t a key_size B.null)
+
+    (* create_in *)
+    (fun () r ->
+       if no_key then unit_to_stateful_key_t a
+       else if U32.(key_size >^ 0ul) then
+         buffer_to_stateful_key_t a key_size (B.malloc r (Lib.IntTypes.u8 0) key_size)
+       else buffer_to_stateful_key_t a key_size B.null)
+
+    (* free *)
+    (fun _ s -> if U32.(key_size >^ 0ul) then B.free (s <: B.buffer uint8) else ())
+
+    (* copy *)
     (fun _ s_src s_dst ->
-      if key_size = 0 then ()
-      else B.blit (s_src <: B.buffer uint8) 0ul
-                  (s_dst <: B.buffer uint8) 0ul (U32.uint_to_t key_size))
+      if U32.(key_size >^ 0ul) then
+        B.blit (s_src <: B.buffer uint8) 0ul
+               (s_dst <: B.buffer uint8) 0ul key_size
+      else ())
 
 inline_for_extraction noextract
-let stateful_key_to_buffer (#a : alg) (#key_size : key_size_ty a)
-                           (key : stateful_key_t a key_size) :
-  b:B.buffer uint8 { B.length b = key_size } =
-  if key_size = 0 then B.null #uint8 else key
+let stateful_key_to_buffer (#a : alg) (#no_key : bool) (#key_size : key_size_t a no_key)
+                           (key : stateful_key_t a no_key key_size) :
+  b:B.buffer uint8 { B.length b = U32.v key_size } =
+  if no_key then B.null #uint8 else key
 
 inline_for_extraction noextract  
 let k = stateful_key
@@ -360,10 +378,11 @@ let update_multi_associative #a key_size () acc prevlen1 prevlen2 input1 input2 
 noextract
 val blake2_hash_incremental_s :
   a : alg ->
-  #key_size : key_size_ty a ->
+  no_key : bool ->
+  key_size : key_size_t a no_key ->
   i:index ->
-  key: I.((k a key_size).t ()) ->
-  input:S.seq uint8 { S.length input <= max_input_length a key_size } ->
+  key: I.((k a no_key key_size).t ()) ->
+  input:S.seq uint8 { S.length input <= max_input_length a (U32.v key_size) } ->
   output:S.seq uint8 { S.length output = output_size a }
 
 noextract
@@ -373,14 +392,14 @@ let size_block_props (a : Spec.alg) :
     Spec.size_block a > 0) = ()
 
 #push-options "--z3cliopt smt.arith.nl=false"
-let blake2_hash_incremental_s a #key_size i key input =
+let blake2_hash_incremental_s a no_key key_size i key input =
   (**) size_block_props a;
   (**) Math.Lemmas.modulo_lemma 0 (Spec.size_block a);
   let bs, l = Spec.Hash.Incremental.split_blocks (to_hash_alg a) input in
-  let acc1 = init_s #a #key_size i key in
-  let acc2 = update_multi_s #a key_size i acc1 0 bs in
-  let acc3 = update_last_s #a key_size i acc2 (S.length bs) l in
-  let acc4 = finish_s #a #key_size i key acc3 in
+  let acc1 = init_s #a #(U32.v key_size) i key in
+  let acc2 = update_multi_s #a (U32.v key_size) i acc1 0 bs in
+  let acc3 = update_last_s #a (U32.v key_size) i acc2 (S.length bs) l in
+  let acc4 = finish_s #a #(U32.v key_size) i key acc3 in
   acc4
 #pop-options
 
@@ -390,59 +409,64 @@ let blake2_hash_incremental_s a #key_size i key input =
 noextract
 val blake2_hash_incremental_s_is_hash_incremental :
   a : alg ->
-  #key_size : key_size_ty a ->
+  no_key : bool ->
+  key_size : key_size_t a no_key ->
   i:index ->
-  key: I.((k a key_size).t ()) ->
-  input:S.seq uint8 { S.length input <= max_input_length a key_size } ->
+  key: I.((k a no_key key_size).t ()) ->
+  input:S.seq uint8 { S.length input <= max_input_length a (U32.v key_size) } ->
   Lemma(
-    blake2_hash_incremental_s a #key_size i key input ==
-      Spec.Hash.Incremental.blake2_hash_incremental (to_hash_alg a) key_size key input)
+    blake2_hash_incremental_s a no_key key_size i key input ==
+      Spec.Hash.Incremental.blake2_hash_incremental (to_hash_alg a) (U32.v key_size) key input)
 
 noextract
 let init_s_blake2_init_eq
   (a : alg)
-  (#key_size : key_size_ty a)
+  (no_key : bool)
+  (key_size : key_size_t a no_key)
   (i:index)
-  (key: I.((k a key_size).t ())) :
+  (key: I.((k a no_key key_size).t ())) :
   Lemma(
-    (init_s #a #key_size i key,
-     Hash.nat_to_extra_state (to_hash_alg a) (blake2_prevlength a key_size 0)) ==
-      Spec.Hash.Incremental.blake2_init (to_hash_alg a) key_size key) =
+    (init_s #a #(U32.v key_size) i key,
+     Hash.nat_to_extra_state (to_hash_alg a) (blake2_prevlength a (U32.v key_size) 0)) ==
+      Spec.Hash.Incremental.blake2_init (to_hash_alg a) (U32.v key_size) key) =
   ()
 
 #push-options "--z3cliopt smt.arith.nl=false"
-let blake2_hash_incremental_s_is_hash_incremental a #key_size i key input =
+let blake2_hash_incremental_s_is_hash_incremental a no_key key_size i key input =
   size_block_props a;
   Math.Lemmas.modulo_lemma 0 (Spec.size_block a);
   let bs, l = Spec.Hash.Incremental.split_blocks (to_hash_alg a) input in
-  let acc1 = init_s #a #key_size i key in
-  let acc2 = update_multi_s key_size i acc1 0 bs in
-  let acc3 = update_last_s key_size i acc2 (S.length bs) l in
-  let acc4 = finish_s #a #key_size i key acc3 in
-  assert(acc4 == blake2_hash_incremental_s a #key_size i key input); (* sanity check *)
-  let s1 = Spec.Hash.Incremental.blake2_init (to_hash_alg a) key_size key in
+  let acc1 = init_s #a #(U32.v key_size) i key in
+  let acc2 = update_multi_s (U32.v key_size) i acc1 0 bs in
+  let acc3 = update_last_s (U32.v key_size) i acc2 (S.length bs) l in
+  let acc4 = finish_s #a #(U32.v key_size) i key acc3 in
+  assert(acc4 == blake2_hash_incremental_s a no_key key_size i key input); (* sanity check *)
+  let s1 = Spec.Hash.Incremental.blake2_init (to_hash_alg a) (U32.v key_size) key in
   let s2 = Agile.update_multi (to_hash_alg a) s1 bs in
   let prevlen = S.length bs in (* dummy value: this variable is actually not used *)
   let s3 = Spec.Hash.Incremental.update_last (to_hash_alg a) s2 prevlen l in
   let s4 = Spec.Hash.PadFinish.finish (to_hash_alg a) s3 in
-  let s4' = Spec.Hash.Incremental.blake2_hash_incremental (to_hash_alg a) key_size key input in
+  let s4' =
+    Spec.Hash.Incremental.blake2_hash_incremental (to_hash_alg a) (U32.v key_size) key input in
   assert(s4 == s4'); (* sanity check *)
   (* The proof *)
   (* 1 *)
-  let es1 = Hash.nat_to_extra_state (to_hash_alg a) (blake2_prevlength a key_size 0) in
+  let es1 = Hash.nat_to_extra_state (to_hash_alg a) (blake2_prevlength a (U32.v key_size) 0) in
   let s1' = (acc1, es1) in
-  init_s_blake2_init_eq a i key;
+  init_s_blake2_init_eq a no_key key_size i key;
   assert(s1' == s1);
   (* 2 *)
   Spec.Hash.Incremental.Lemmas.update_multi_extra_state_eq (to_hash_alg a) s1 bs;
-  Spec.Hash.Lemmas.extra_state_v_of_nat (to_hash_alg a) (blake2_prevlength a key_size 0);
+  Spec.Hash.Lemmas.extra_state_v_of_nat (to_hash_alg a) (blake2_prevlength a (U32.v key_size) 0);
   assert(Hash.extra_state_v es1 + S.length bs <= Hash.max_extra_state (to_hash_alg a));
   Spec.Hash.Lemmas.extra_state_add_nat_bound_lem2 #(to_hash_alg a) es1 (S.length bs);
-  let es2 = Hash.nat_to_extra_state (to_hash_alg a) (blake2_prevlength a key_size (S.length bs)) in
+  let es2 = Hash.nat_to_extra_state (to_hash_alg a)
+                                    (blake2_prevlength a (U32.v key_size) (S.length bs)) in
   let s2' = (acc2, es2) in
-  blake2_prevlength_add_right_eq a key_size 0 (S.length bs);
+  blake2_prevlength_add_right_eq a (U32.v key_size) 0 (S.length bs);
   add_zero_left_is_same (S.length bs);
-  assert(blake2_prevlength a key_size 0 + S.length bs = blake2_prevlength a key_size (S.length bs));
+  assert(blake2_prevlength a (U32.v key_size) 0 + S.length bs =
+         blake2_prevlength a (U32.v key_size) (S.length bs));
   assert(s2' == s2);
   (* 3 *)
   let es3 = Hash.nat_to_extra_state (to_hash_alg a) 0 in
@@ -456,26 +480,27 @@ let blake2_hash_incremental_s_is_hash_incremental a #key_size i key input =
 noextract
 val spec_is_incremental:
   a : alg ->
-  #key_size : key_size_ty a ->
+  no_key : bool ->
+  key_size : key_size_t a no_key ->
   i:index ->
-  key: I.((k a key_size).t ()) ->
-  input:S.seq uint8 { S.length input <= max_input_length a key_size } ->
+  key: I.((k a no_key key_size).t ()) ->
+  input:S.seq uint8 { S.length input <= max_input_length a (U32.v key_size) } ->
   Lemma (
     (**) size_block_props a;
     (**) Math.Lemmas.modulo_lemma 0 (Spec.size_block a);
     let bs, l = Lib.UpdateMulti.split_at_last_lazy (U32.v (block_len a)) input in
-    let hash0 = init_s #a #key_size i key in
-    let hash1 = update_multi_s key_size i hash0 0 bs in
-    let hash2 = update_last_s key_size i hash1 (S.length bs) l in
-    let hash3 = finish_s #a #key_size i key hash2 in
-    hash3 `S.equal` spec_s a #key_size i key input)
+    let hash0 = init_s #a #(U32.v key_size) i key in
+    let hash1 = update_multi_s (U32.v key_size) i hash0 0 bs in
+    let hash2 = update_last_s (U32.v key_size) i hash1 (S.length bs) l in
+    let hash3 = finish_s #a #(U32.v key_size) i key hash2 in
+    hash3 `S.equal` spec_s a #(U32.v key_size) i key input)
 #pop-options
 
 #push-options "--z3cliopt smt.arith.nl=false"
-let spec_is_incremental a #key_size i key input =
-  blake2_hash_incremental_s_is_hash_incremental a i key input;
+let spec_is_incremental a no_key key_size i key input =
+  blake2_hash_incremental_s_is_hash_incremental a no_key key_size i key input;
   (**) size_block_props a;
-  Spec.Hash.Incremental.blake2_is_hash_incremental (to_hash_alg a) key_size key input
+  Spec.Hash.Incremental.blake2_is_hash_incremental (to_hash_alg a) (U32.v key_size) key input
 #pop-options
 
 noextract
@@ -583,14 +608,15 @@ inline_for_extraction noextract
 val mk_update_multi:
   a : alg ->
   m : m_spec ->
-  key_size : key_size_ty a ->
+  no_key : bool ->
+  key_size : key_size_t a no_key ->
   (i:G.erased index -> (
   let i = G.reveal i in
   s:s a m ->
   prevlen:U64.t { U64.v prevlen % U32.v (block_len a) = 0 } ->
   blocks:B.buffer uint8 { B.length blocks % U32.v (block_len a) = 0 } ->
   len: U32.t { U32.v len = B.length blocks /\
-               U64.v prevlen + U32.v len <= max_input_length a key_size } ->
+               U64.v prevlen + U32.v len <= max_input_length a (U32.v key_size) } ->
   ST.Stack unit
   (requires fun h0 ->
     let state = stateful_blake2 a m in
@@ -602,12 +628,12 @@ val mk_update_multi:
     B.(modifies (state.I.footprint #i h0 s) h0 h1) /\
     state.I.footprint #i h0 s == state.I.footprint #i h1 s /\
     state.I.invariant #i h1 s /\
-    state.I.v i h1 s == update_multi_s #a key_size i (state.I.v i h0 s) (U64.v prevlen)
+    state.I.v i h1 s == update_multi_s #a (U32.v key_size) i (state.I.v i h0 s) (U64.v prevlen)
                                                   (B.as_seq h0 blocks) /\
     (state.I.freeable #i h0 s ==> state.I.freeable #i h1 s))))
 
 #push-options "--z3cliopt smt.arith.nl=false"
-let mk_update_multi a m key_size i acc prevlen blocks len =
+let mk_update_multi a m no_key key_size i acc prevlen blocks len =
   (**) size_block_props a;
   [@inline_let] let wv = get_wv acc in
   [@inline_let] let h = get_state_p acc in
@@ -615,7 +641,7 @@ let mk_update_multi a m key_size i acc prevlen blocks len =
   let nb = U32.(len /^ block_len a) in
   (**) Math.Lemmas.div_exact_r (U32.v len) (U32.v (block_len a));
   (**) Math.Lemmas.multiply_fractions (U32.v len) (U32.v (block_len a));
-  [@inline_let] let prevlen' = blake2_prevlen a (U32.uint_to_t key_size) prevlen in
+  [@inline_let] let prevlen' = blake2_prevlen a key_size prevlen in
   (**) assert(Lib.Buffer.disjoint wv h);
   Impl.blake2_update_multi #a #m #len (Impl.blake2_update_block #a #m) wv h
                            prevlen' blocks nb;
@@ -627,9 +653,9 @@ let mk_update_multi a m key_size i acc prevlen blocks len =
   (**)                  (s_v h0 acc));
   (**) state_types_equalities a;
   (**) assert(Spec.Blake2.state a == Hash.words_state' (to_hash_alg a));
-  (**) update_multi_eq key_size (U32.v nb) (s_v h0 acc) (U64.v prevlen) (B.as_seq h0 blocks);
-  (**) assert(Lib.IntTypes.uint_v prevlen' = blake2_prevlength a key_size (U64.v prevlen));
-  (**) assert(s_v h3 acc == update_multi_s key_size () (s_v h0 acc) (U64.v prevlen) (B.as_seq h0 blocks));
+  (**) update_multi_eq (U32.v key_size) (U32.v nb) (s_v h0 acc) (U64.v prevlen) (B.as_seq h0 blocks);
+  (**) assert(Lib.IntTypes.uint_v prevlen' = blake2_prevlength a (U32.v key_size) (U64.v prevlen));
+  (**) assert(s_v h3 acc == update_multi_s (U32.v key_size) () (s_v h0 acc) (U64.v prevlen) (B.as_seq h0 blocks));
   (**) assert(B.(modifies ((stateful_blake2 a m).I.footprint #() h0 acc) h0 h3))
 #pop-options
 
@@ -637,7 +663,8 @@ inline_for_extraction noextract
 val mk_update_last:
   a : alg ->
   m : m_spec ->
-  key_size : key_size_ty a ->
+  no_key : bool ->
+  key_size : key_size_t a no_key ->
   (i: G.erased index -> (
   let i = G.reveal i in
   s:s a m ->
@@ -646,7 +673,7 @@ val mk_update_last:
   last_len:U32.t{
     last_len = B.len last /\
     U32.v last_len <= U32.v (block_len a) /\
-    U64.v prevlen + U32.v last_len <= max_input_length a key_size} ->
+    U64.v prevlen + U32.v last_len <= max_input_length a (U32.v key_size)} ->
   ST.Stack unit
   (requires fun h0 ->
     let state = stateful_blake2 a m in
@@ -656,7 +683,7 @@ val mk_update_last:
   (ensures fun h0 _ h1 ->
     let state = stateful_blake2 a m in
     state.I.invariant #i h1 s /\
-    state.I.v i h1 s == update_last_s #a key_size i (state.I.v i h0 s)
+    state.I.v i h1 s == update_last_s #a (U32.v key_size) i (state.I.v i h0 s)
                                       (U64.v prevlen) (B.as_seq h0 last) /\
     B.(modifies (state.I.footprint #i h0 s) h0 h1) /\
     state.I.footprint #i h0 s == state.I.footprint #i h1 s /\
@@ -664,21 +691,21 @@ val mk_update_last:
 
 /// TODO: after analysis with quake, this proof sometimes loops
 #push-options "--ifuel 1 --z3cliopt smt.arith.nl=false"
-let mk_update_last a m key_size i acc prevlen last last_len =
+let mk_update_last a m no_key key_size i acc prevlen last last_len =
   (**) size_block_props a;
   [@inline_let] let wv = get_wv acc in
   [@inline_let] let h = get_state_p acc in
   (**) let h0 = ST.get () in
   (**) assert_norm(U64.v prevlen + U32.v last_len <= Spec.Blake2.max_limb a);
   [@inline_let]
-  let prevlen' = blake2_prevlen a (U32.uint_to_t key_size) prevlen in
+  let prevlen' = blake2_prevlen a key_size prevlen in
   (**) assert((U64.v prevlen) % Hash.block_length (to_hash_alg a) = 0);
   (**) assert(B.length last <= Hash.block_length (to_hash_alg a));
-  (**) assert(U64.v prevlen + B.length last <= max_input_length a key_size);
+  (**) assert(U64.v prevlen + B.length last <= max_input_length a (U32.v key_size));
   Impl.blake2_update_last #a #m (Impl.blake2_update_block #a #m) #last_len
                           wv h prevlen' last_len last;
   (* TODO: SH: if not put at the proper place, this call makes the proof loop or randomly fail *)
-  (**) update_last_eq key_size (U64.v prevlen) (B.as_seq h0 last) (s_v h0 acc);
+  (**) update_last_eq (U32.v key_size) (U64.v prevlen) (B.as_seq h0 last) (s_v h0 acc);
   (**) let h2 = ST.get () in
   (**) assert(
   (**)   Core.state_v h2 h ==
@@ -686,37 +713,36 @@ let mk_update_last a m key_size i acc prevlen last last_len =
   (**)                               (B.as_seq h0 last)
   (**)                               (Core.state_v h0 h));
   (**) assert(s_v h2 acc ==
-  (**)   update_last_s key_size () (s_v h0 acc) (U64.v prevlen) (B.as_seq h0 last))
+  (**)   update_last_s (U32.v key_size) () (s_v h0 acc) (U64.v prevlen) (B.as_seq h0 last))
 #pop-options
 
-/// Pay attention to the fact that the ``key_size`` parameter is not Low* and
-/// appears in extracted code (in some tests which must be reduced, for the definition
-/// of the key type, for some arithmetic and for the size of the buffer to allocate
-/// for the key): it must thus be a constant.
 #push-options "--ifuel 1 --z3cliopt smt.arith.nl=false"
 inline_for_extraction noextract
-let blake2 (a : alg) (m : m_spec) (key_size : key_size_ty a) : I.block unit =
+let blake2 (a : alg) (m : m_spec) (no_key : bool) (key_size : key_size_t a no_key)
+//  I.block unit
+  =
   I.Block
     I.Erased (* key management *)
     
     (stateful_blake2 a m) (* state *)
-    (k a key_size) (* key *)
+    (k a no_key key_size) (* key *)
     
     (fun () -> max_input_length a (Spec.max_key a)) (* max_input_length *)
     (fun () -> output_len a) (* output_len *)
     (fun () -> block_len a) (* block_len *)
     
-    (fun () k -> init_s #a #key_size () k) (* init_s *)
-    (fun () acc prevlen input -> update_multi_s key_size () acc prevlen input) (* update_multi_s *)
-    (fun () acc prevlen input -> update_last_s key_size () acc prevlen input) (* update_last_s *)
-    (fun () k acc -> finish_s #a #key_size () k acc) (* finish_s *)
-    (fun () -> spec_s a #key_size ()) (* spec_s *)
+    (fun () k -> init_s #a #(U32.v key_size) () k) (* init_s *)
+    (fun () acc prevlen input -> update_multi_s (U32.v key_size) () acc prevlen input) (* update_multi_s *)
+    (fun () acc prevlen input -> update_last_s (U32.v key_size) () acc prevlen input) (* update_last_s *)
+    (fun () k acc -> finish_s #a #(U32.v key_size) () k acc) (* finish_s *)
+    (fun () -> spec_s a #(U32.v key_size) ()) (* spec_s *)
 
-    (fun () prevlen acc -> update_multi_zero key_size () prevlen acc) (* update_multi_zero *)
+    (* update_multi_zero *)
+    (fun () prevlen acc -> update_multi_zero (U32.v key_size) () prevlen acc)
     (* update_multi_associative *)
     (fun () acc prevlen1 prevlen2 input1 input2 ->
-      update_multi_associative key_size () acc prevlen1 prevlen2 input1 input2)
-    (fun () k input -> spec_is_incremental a #key_size () k input) (* spec_is_incremental *)
+      update_multi_associative (U32.v key_size) () acc prevlen1 prevlen2 input1 input2)
+    (fun () k input -> spec_is_incremental a no_key key_size () k input) (* spec_is_incremental *)
     (fun _ acc -> ()) (* index_of_state *)
 
     (* init *)
@@ -724,18 +750,18 @@ let blake2 (a : alg) (m : m_spec) (key_size : key_size_ty a) : I.block unit =
       [@inline_let] let wv = get_wv acc in
       [@inline_let] let h = get_state_p acc in
       [@inline_let]
-      let key : b:B.buffer uint8{B.length b = key_size} =
-        if key_size = 0 then B.null #uint8 else key in
+      let key : b:B.buffer uint8{B.length b = U32.v key_size} =
+        if no_key then B.null #uint8 else key in
       Impl.blake2_init #a #m (Impl.blake2_update_block #a #m) wv h
-                       (U32.uint_to_t key_size) key
+                       key_size key
                        (output_len a))
 
     (* update_multi *)
-    (fun _ acc prevlen blocks len -> mk_update_multi a m key_size () acc prevlen blocks len)
+    (fun _ acc prevlen blocks len -> mk_update_multi a m no_key key_size () acc prevlen blocks len)
 
     (* update_last *)
     (fun _ acc prevlen last last_len ->
-      mk_update_last a m key_size () acc prevlen last last_len)
+      mk_update_last a m no_key key_size () acc prevlen last last_len)
 
     (* finish *)
     (fun _ k acc dst ->
@@ -747,81 +773,81 @@ let blake2 (a : alg) (m : m_spec) (key_size : key_size_ty a) : I.block unit =
 /// The incremental hash functions instantiations. Note that we can't write a
 /// generic one, because the normalization then performed by Kremlin explodes.
 inline_for_extraction noextract
-let mk_blake2s_32_create_in (key_size : key_size_ty Spec.Blake2S) =
-  F.create_in (blake2 Spec.Blake2S M32 key_size) () (s Spec.Blake2S M32)
-              (I.optional_key () I.Erased (k Spec.Blake2S key_size))
+let mk_blake2s_32_create_in (no_key : bool) (key_size : key_size_t Spec.Blake2S no_key) =
+  F.create_in (blake2 Spec.Blake2S M32 no_key key_size) () (s Spec.Blake2S M32)
+              (I.optional_key () I.Erased (k Spec.Blake2S no_key key_size))
 
 inline_for_extraction noextract
-let mk_blake2s_32_update (key_size : key_size_ty Spec.Blake2S) =
-  F.update (blake2 Spec.Blake2S M32 key_size) (G.hide ()) (s Spec.Blake2S M32)
-           (I.optional_key () I.Erased (k Spec.Blake2S key_size))
+let mk_blake2s_32_update (no_key : bool) (key_size : key_size_t Spec.Blake2S no_key) =
+  F.update (blake2 Spec.Blake2S M32 no_key key_size) (G.hide ()) (s Spec.Blake2S M32)
+           (I.optional_key () I.Erased (k Spec.Blake2S no_key key_size))
 
 inline_for_extraction noextract
-let mk_blake2s_32_blake2s_32_finish (key_size : key_size_ty Spec.Blake2S) =
-  F.mk_finish (blake2 Spec.Blake2S M32 key_size) () (s Spec.Blake2S M32)
-              (I.optional_key () I.Erased (k Spec.Blake2S key_size))
+let mk_blake2s_32_blake2s_32_finish (no_key : bool) (key_size : key_size_t Spec.Blake2S no_key) =
+  F.mk_finish (blake2 Spec.Blake2S M32 no_key key_size) () (s Spec.Blake2S M32)
+              (I.optional_key () I.Erased (k Spec.Blake2S no_key key_size))
 
 inline_for_extraction noextract
-let mk_blake2s_32_free (key_size : key_size_ty Spec.Blake2S) =
-  F.free (blake2 Spec.Blake2S M32 key_size) (G.hide ()) (s Spec.Blake2S M32)
-         (I.optional_key () I.Erased (k Spec.Blake2S key_size))
+let mk_blake2s_32_free (no_key : bool) (key_size : key_size_t Spec.Blake2S no_key) =
+  F.free (blake2 Spec.Blake2S M32 no_key key_size) (G.hide ()) (s Spec.Blake2S M32)
+         (I.optional_key () I.Erased (k Spec.Blake2S no_key key_size))
 
 inline_for_extraction noextract
-let mk_blake2s_128_create_in (key_size : key_size_ty Spec.Blake2S) =
-  F.create_in (blake2 Spec.Blake2S M128 key_size) () (s Spec.Blake2S M128)
-              (I.optional_key () I.Erased (k Spec.Blake2S key_size))
+let mk_blake2s_128_create_in (no_key : bool) (key_size : key_size_t Spec.Blake2S no_key) =
+  F.create_in (blake2 Spec.Blake2S M128 no_key key_size) () (s Spec.Blake2S M128)
+              (I.optional_key () I.Erased (k Spec.Blake2S no_key key_size))
 
 inline_for_extraction noextract
-let mk_blake2s_128_update (key_size : key_size_ty Spec.Blake2S) =
-  F.update (blake2 Spec.Blake2S M128 key_size) (G.hide ()) (s Spec.Blake2S M128)
-           (I.optional_key () I.Erased (k Spec.Blake2S key_size))
+let mk_blake2s_128_update (no_key : bool) (key_size : key_size_t Spec.Blake2S no_key) =
+  F.update (blake2 Spec.Blake2S M128 no_key key_size) (G.hide ()) (s Spec.Blake2S M128)
+           (I.optional_key () I.Erased (k Spec.Blake2S no_key key_size))
 
 inline_for_extraction noextract
-let mk_blake2s_128_blake2s_128_finish (key_size : key_size_ty Spec.Blake2S) =
-  F.mk_finish (blake2 Spec.Blake2S M128 key_size) () (s Spec.Blake2S M128)
-              (I.optional_key () I.Erased (k Spec.Blake2S key_size))
+let mk_blake2s_128_blake2s_128_finish (no_key : bool) (key_size : key_size_t Spec.Blake2S no_key) =
+  F.mk_finish (blake2 Spec.Blake2S M128 no_key key_size) () (s Spec.Blake2S M128)
+              (I.optional_key () I.Erased (k Spec.Blake2S no_key key_size))
 
 inline_for_extraction noextract
-let mk_blake2s_128_free (key_size : key_size_ty Spec.Blake2S) =
-  F.free (blake2 Spec.Blake2S M128 key_size) (G.hide ()) (s Spec.Blake2S M128)
-         (I.optional_key () I.Erased (k Spec.Blake2S key_size))
+let mk_blake2s_128_free (no_key : bool) (key_size : key_size_t Spec.Blake2S no_key) =
+  F.free (blake2 Spec.Blake2S M128 no_key key_size) (G.hide ()) (s Spec.Blake2S M128)
+         (I.optional_key () I.Erased (k Spec.Blake2S no_key key_size))
 
 inline_for_extraction noextract
-let mk_blake2b_32_create_in (key_size : key_size_ty Spec.Blake2B) =
-  F.create_in (blake2 Spec.Blake2B M32 key_size) () (s Spec.Blake2B M32)
-              (I.optional_key () I.Erased (k Spec.Blake2B key_size))
+let mk_blake2b_32_create_in (no_key : bool) (key_size : key_size_t Spec.Blake2B no_key) =
+  F.create_in (blake2 Spec.Blake2B M32 no_key key_size) () (s Spec.Blake2B M32)
+              (I.optional_key () I.Erased (k Spec.Blake2B no_key key_size))
 
 inline_for_extraction noextract
-let mk_blake2b_32_update (key_size : key_size_ty Spec.Blake2B) =
-  F.update (blake2 Spec.Blake2B M32 key_size) (G.hide ()) (s Spec.Blake2B M32)
-           (I.optional_key () I.Erased (k Spec.Blake2B key_size))
+let mk_blake2b_32_update (no_key : bool) (key_size : key_size_t Spec.Blake2B no_key) =
+  F.update (blake2 Spec.Blake2B M32 no_key key_size) (G.hide ()) (s Spec.Blake2B M32)
+           (I.optional_key () I.Erased (k Spec.Blake2B no_key key_size))
 
 inline_for_extraction noextract
-let mk_blake2b_32_blake2b_32_finish (key_size : key_size_ty Spec.Blake2B) =
-  F.mk_finish (blake2 Spec.Blake2B M32 key_size) () (s Spec.Blake2B M32)
-              (I.optional_key () I.Erased (k Spec.Blake2B key_size))
+let mk_blake2b_32_blake2b_32_finish (no_key : bool) (key_size : key_size_t Spec.Blake2B no_key) =
+  F.mk_finish (blake2 Spec.Blake2B M32 no_key key_size) () (s Spec.Blake2B M32)
+              (I.optional_key () I.Erased (k Spec.Blake2B no_key key_size))
 
 inline_for_extraction noextract
-let mk_blake2b_32_free (key_size : key_size_ty Spec.Blake2B) =
-  F.free (blake2 Spec.Blake2B M32 key_size) (G.hide ()) (s Spec.Blake2B M32)
-         (I.optional_key () I.Erased (k Spec.Blake2B key_size))
+let mk_blake2b_32_free (no_key : bool) (key_size : key_size_t Spec.Blake2B no_key) =
+  F.free (blake2 Spec.Blake2B M32 no_key key_size) (G.hide ()) (s Spec.Blake2B M32)
+         (I.optional_key () I.Erased (k Spec.Blake2B no_key key_size))
 
 inline_for_extraction noextract
-let mk_blake2b_256_create_in (key_size : key_size_ty Spec.Blake2B) =
-  F.create_in (blake2 Spec.Blake2B M256 key_size) () (s Spec.Blake2B M256)
-              (I.optional_key () I.Erased (k Spec.Blake2B key_size))
+let mk_blake2b_256_create_in (no_key : bool) (key_size : key_size_t Spec.Blake2B no_key) =
+  F.create_in (blake2 Spec.Blake2B M256 no_key key_size) () (s Spec.Blake2B M256)
+              (I.optional_key () I.Erased (k Spec.Blake2B no_key key_size))
 
 inline_for_extraction noextract
-let mk_blake2b_256_update (key_size : key_size_ty Spec.Blake2B) =
-  F.update (blake2 Spec.Blake2B M256 key_size) (G.hide ()) (s Spec.Blake2B M256)
-           (I.optional_key () I.Erased (k Spec.Blake2B key_size))
+let mk_blake2b_256_update (no_key : bool) (key_size : key_size_t Spec.Blake2B no_key) =
+  F.update (blake2 Spec.Blake2B M256 no_key key_size) (G.hide ()) (s Spec.Blake2B M256)
+           (I.optional_key () I.Erased (k Spec.Blake2B no_key key_size))
 
 inline_for_extraction noextract
-let mk_blake2b_256_blake2b_256_finish (key_size : key_size_ty Spec.Blake2B) =
-  F.mk_finish (blake2 Spec.Blake2B M256 key_size) () (s Spec.Blake2B M256)
-              (I.optional_key () I.Erased (k Spec.Blake2B key_size))
+let mk_blake2b_256_blake2b_256_finish (no_key : bool) (key_size : key_size_t Spec.Blake2B no_key) =
+  F.mk_finish (blake2 Spec.Blake2B M256 no_key key_size) () (s Spec.Blake2B M256)
+              (I.optional_key () I.Erased (k Spec.Blake2B no_key key_size))
 
 inline_for_extraction noextract
-let mk_blake2b_256_free (key_size : key_size_ty Spec.Blake2B) =
-  F.free (blake2 Spec.Blake2B M256 key_size) (G.hide ()) (s Spec.Blake2B M256)
-         (I.optional_key () I.Erased (k Spec.Blake2B key_size))
+let mk_blake2b_256_free (no_key : bool) (key_size : key_size_t Spec.Blake2B no_key) =
+  F.free (blake2 Spec.Blake2B M256 no_key key_size) (G.hide ()) (s Spec.Blake2B M256)
+         (I.optional_key () I.Erased (k Spec.Blake2B no_key key_size))
